src/impl/TLS13.Connection.External.fsti
@@ -78,38 +78,26 @@ fn client_write_raw_record
           pts_to header 'header_bytes **
           pts_to cipher 'cipher_bytes
 
-fn client_read_raw_record_header
+fn client_read_raw
   (c: connection)
   (ch: IO.channel)
-  (header: array U8.t)
-  (header_len: SZ.t)
+  (buf: array U8.t)
+  (total_len: SZ.t)
+  (offset: SZ.t)
+  (remaining: SZ.t)
   requires   is_connection c **
   IO.is_channel ch **
-  pts_to header 'old_header **
-  pure (B.length 'old_header == SZ.v header_len /\
-        SZ.v header_len == 5)
-  returns ok: bool
-  ensures exists* header_bytes.
+  pts_to buf 'old **
+  pure (B.length 'old == SZ.v total_len /\
+        SZ.v remaining > 0 /\
+        SZ.v offset + SZ.v remaining <= SZ.v total_len)
+  returns n: SZ.t
+  ensures exists* bytes.
           is_connection c **
           IO.is_channel ch **
-          pts_to header header_bytes **
-          pure (B.length header_bytes == 5)
-
-fn client_read_raw_record_fragment
-  (c: connection)
-  (ch: IO.channel)
-  (cipher: array U8.t)
-  (cipher_len: SZ.t)
-  requires   is_connection c **
-  IO.is_channel ch **
-  pts_to cipher 'old_cipher **
-  pure (B.length 'old_cipher == SZ.v cipher_len)
-  returns ok: bool
-  ensures exists* cipher_bytes.
-          is_connection c **
-          IO.is_channel ch **
-          pts_to cipher cipher_bytes **
-          pure (B.length cipher_bytes == SZ.v cipher_len)
+          pts_to buf bytes **
+          pure (B.length bytes == SZ.v total_len /\
+                SZ.v n <= SZ.v remaining)
 
 fn client_close (c: connection) (ch: IO.channel)
   requires is_connection c ** IO.is_channel ch
